Re-add exponential fractions to prove list equiv insert

arrays/inv/list_equiv.v
@@ -18,10 +18,18 @@ Module ListEquiv (Params: SKIP_LIST_PARAMS).
   Section Proofs.
     Context `{!heapGS Σ, !lockG Σ} (lvl: Z).
 
-    Definition nodeN (rep: node_rep) := nroot .@ "node" .@ rep.
+    Definition nodeN (l: loc) := nroot .@ "node" .@ l.
 
     Definition node_inv(s: loc) (succ: node_rep) : iProp Σ := 
       s ↦{#1 / 2} rep_to_node succ.
+
+    Fixpoint exp2 (n: nat) : frac :=
+      match n with
+      | O => 1
+      | S n => 2 * exp2 n
+      end.
+
+    Definition lfrac : frac := 1 / exp2 (Z.to_nat (lvl + 2)).
 
     Definition in_lock (next: loc) : iProp Σ := 
       ∃ (vs: list val), next ↦∗{#1 / 2} vs.
@@ -34,14 +42,18 @@ Module ListEquiv (Params: SKIP_LIST_PARAMS).
         | nil => ∃ (γ: gname) (t: loc), 
                  (node_next pred +ₗ lvl) ↦{#1 / 2} #t
                  ∗
-                 inv (nodeN tail) (node_inv t tail)
+                 inv (nodeN t) (node_inv t tail)
+                 ∗
+                 t ↦{#lfrac} rep_to_node tail
                  ∗
                  is_lock γ (node_lock pred) (in_lock (node_next pred))
 
         | succ :: _ => ∃ (γ: gname) (s: loc), 
                        (node_next pred +ₗ lvl) ↦{#1 / 2} #s
                        ∗
-                       inv (nodeN succ) (node_inv s succ)
+                       inv (nodeN s) (node_inv s succ)
+                       ∗
+                       s ↦{#lfrac} rep_to_node succ
                        ∗
                        is_lock γ (node_lock pred) (in_lock (node_next pred))
                        ∗
@@ -59,7 +71,8 @@ Module ListEquiv (Params: SKIP_LIST_PARAMS).
     Proof.
       destruct L as [|n].
       + iIntros "Hrep". by iFrame.
-      + iIntros "Hlist". iDestruct "Hlist" as (γ s) "(Hpt & Hs & Hlock & HP & Hmatch)".
+      + iIntros "Hlist". 
+        iDestruct "Hlist" as (γ s) "(Hpt & Hinvs & Hs & Hlock & HP & Hmatch)".
         iFrame. iIntros "Hlist". iFrame.
         iExists γ, s. iFrame.
     Qed.
@@ -71,7 +84,7 @@ Module ListEquiv (Params: SKIP_LIST_PARAMS).
         ∃ (γ: gname) (s: loc),
           (node_next pred +ₗ lvl) ↦{#1 / 2} #s
           ∗
-          inv (nodeN succ) (node_inv s succ)
+          inv (nodeN s) (node_inv s succ)
           ∗
           is_lock γ (node_lock pred) (in_lock (node_next pred))
           ∗
@@ -84,13 +97,13 @@ Module ListEquiv (Params: SKIP_LIST_PARAMS).
         destruct L as [|curr L].
         - inversion HL'; subst.
           iIntros "Hlist".
-          iDestruct "Hlist" as (γ t) "(Hpt & #Ht & #Hlock)".
+          iDestruct "Hlist" as (γ t) "(Hpt & #Hinvt & Ht & #Hlock)".
           iExists γ, t. iFrame "# ∗".
           iIntros "Hpt". 
           iExists γ, t. iFrame "# ∗".
         - inversion HL'; subst.
           iIntros "Hlist". 
-          iDestruct "Hlist" as (γ s) "(Hpt & #Hs & #Hlock & Hmatch)".
+          iDestruct "Hlist" as (γ s) "(Hpt & #Hinvs & Hs & #Hlock & Hmatch)".
           iExists γ, s. iFrame "# ∗".
           iIntros "Hpt". 
           iExists γ, s. iFrame "# ∗".
@@ -111,7 +124,7 @@ Module ListEquiv (Params: SKIP_LIST_PARAMS).
         iIntros "Hlist".
         iPoseProof (list_equiv_cons with "Hlist") as "(Hlist & Himp)".
         iPoseProof (IHL1 with "Hlist") as "Hlist"; auto.
-        iDestruct "Hlist" as (γ s) "(Hpt & #Hs & Hlock & Himp')".
+        iDestruct "Hlist" as (γ s) "(Hpt & #Hinvs & Hlock & Himp')".
         iExists γ, s. iFrame "# ∗". 
         iIntros "Hpt".
         iApply "Himp". iApply "Himp'". iFrame.
@@ -128,42 +141,50 @@ Module ListEquiv (Params: SKIP_LIST_PARAMS).
           ∗
           (node_next pred +ₗ lvl) ↦{#1/2} #s
           ∗
-          inv (nodeN succ) (node_inv s succ)
+          inv (nodeN s) (node_inv s succ)
+          ∗
+          s ↦{#lfrac} rep_to_node succ
           ∗ 
           is_lock γ (node_lock pred) (in_lock (node_next pred))
           ∗
           P pred
           ∗
-          ((node_next pred +ₗ lvl) ↦{#1/2} #s ∗ P pred -∗ list_equiv ([head] ++ L) P).
+          ((node_next pred +ₗ lvl) ↦{#1/2} #s 
+            ∗ 
+            s ↦{#lfrac} rep_to_node succ
+            ∗ 
+            P pred 
+            -∗ 
+              list_equiv ([head] ++ L) P).
     Proof.
       iIntros (Hin) "Hlist".
       iRevert (head Hin) "Hlist".
       iInduction L as [|succ L] "IHL"; iIntros (head) "Hin"; first by iExFalso.
       iDestruct "Hin" as "[%Heq|Hin]"; subst; iIntros "Hlist".
-      + iDestruct "Hlist" as (γ s) "(Hpt & #Hs & #Hlock & HP & Hlist)".
-        destruct L as [|succ' L]; subst.
-        - iDestruct "Hlist" as (γ' t) "(Hpt' & #Ht & #Hlock')".
+      + iDestruct "Hlist" as (γ s) "(Hpt & #Hinvs & Hs & #Hlock & HP & Hlist)".
+        destruct L as [|next L]; subst.
+        - iDestruct "Hlist" as (γ' t) "(Hpt' & #Hinvt & Ht & #Hlock')".
           iExists t, tail, [head], nil, γ'. iFrame "# ∗".
           iSplit; first by iRight. iSplit; first done.
-          iIntros "(Hpt' & HP)". 
+          iIntros "(Hpt' & Hs' & HP)". 
           iExists γ, s. iFrame "# ∗".
           iExists γ', t. iFrame "# ∗".
-        - iDestruct "Hlist" as (γ' s') "(Hpt' & #Hs' & #Hlock' & Hmatch)".
-          iExists s', succ', [head], (L ++ [tail]), γ'. iFrame "# ∗".
+        - iDestruct "Hlist" as (γ' n) "(Hpt' & #Hinvs' & Hn & #Hlock' & Hmatch)".
+          iExists n, next, [head], (L ++ [tail]), γ'. iFrame "# ∗".
           iSplit; first by iLeft; iRight; iLeft. iSplit; first done.
-          iIntros "(Hpt' & HP)". 
+          iIntros "(Hpt' & Hn' & HP)". 
           iExists γ, s. iFrame "# ∗".
-          iExists γ', s'. iFrame "# ∗".
+          iExists γ', n. iFrame "# ∗".
       + iPoseProof (list_equiv_cons with "Hlist") as "(Hlist & Himp)".
         iPoseProof ("IHL" with "Hin") as "Himp'".
         iPoseProof ("Himp'" with "Hlist") as "Hlist".
-        iDestruct "Hlist" as (s' succ' L1 L2 γ) "(%Hsucc' & %Hsplit & Hpt & #Hs' & Hlock & HP & Himp')".
-        iExists s', succ', ([head] ++ L1), L2, γ. iFrame "# ∗".
+        iDestruct "Hlist" as (n next L1 L2 γ) "(%Hnext & %Hsplit & Hpt & #Hinvn & Hn & #Hlock & HP & Himp')".
+        iExists n, next, ([head] ++ L1), L2, γ. iFrame "# ∗".
         iSplit.
-        { iPureIntro. destruct Hsucc'; first left; by right. }
+        { iPureIntro; destruct Hnext; first left; by right. }
         iSplit.
         { iPureIntro; simpl in *; by rewrite Hsplit. }
-        iIntros "(Hpt' & HP)". 
+        iIntros "(Hpt & Hn & HP)". 
         iApply "Himp". iApply "Himp'". iFrame.
     Qed.
 
@@ -178,29 +199,148 @@ Module ListEquiv (Params: SKIP_LIST_PARAMS).
           ∗
           (node_next pred +ₗ lvl) ↦{#1/2} #s
           ∗
-          inv (nodeN succ) (node_inv s succ)
+          inv (nodeN s) (node_inv s succ)
+          ∗
+          s ↦{#lfrac} rep_to_node succ
           ∗ 
           is_lock γ (node_lock pred) (in_lock (node_next pred))
           ∗
-          ((node_next pred +ₗ lvl) ↦{#1/2} #s -∗ list_equiv ([head] ++ L) P).
+          ((node_next pred +ₗ lvl) ↦{#1/2} #s 
+            ∗ 
+            s ↦{#lfrac} rep_to_node succ
+            -∗ 
+              list_equiv ([head] ++ L) P).
     Proof.
       intros Hin; destruct Hin as [Heq|Hin]; first subst.
-      + iIntros "Hlist". destruct L as [|succ' L].
-        - iDestruct "Hlist" as (γ t) "(Hpt & #Ht & #Hlock)".
+      + iIntros "Hlist". destruct L as [|next L].
+        - iDestruct "Hlist" as (γ t) "(Hpt & #Hinvt & Ht & #Hlock)".
           iExists t, tail, nil, nil, γ. iFrame "# ∗".
           iSplit; first by iRight. iSplit; first done.
-          iIntros "Hpt". 
+          iIntros "(Hpt & Ht)". 
           iExists γ, t. iFrame "# ∗".
-        - iDestruct "Hlist" as (γ s') "(Hpt & #Hs' & #Hlock & ?)".
-          iExists s', succ', nil, (L ++ [tail]), γ. iFrame "# ∗".
+        - iDestruct "Hlist" as (γ n) "(Hpt & #Hinvn & Hn & #Hlock & ?)".
+          iExists n, next, nil, (L ++ [tail]), γ. iFrame "# ∗".
           iSplit; first by repeat iLeft. iSplit; first done.
-          iIntros "Hpt". 
-          iExists γ, s'. iFrame "# ∗".
+          iIntros "(Hpt & Hn)". 
+          iExists γ, n. iFrame "# ∗".
       + iIntros "Hlist".
         iPoseProof (list_equiv_invert_L with "Hlist") as "Hlist"; first done.
-        iDestruct "Hlist" as (s succ L1 L2 γ) "(? & ? & ? & ? & ? & ? & Himp)".
+        iDestruct "Hlist" as (s succ L1 L2 γ) "(? & ? & ? & ? & ? & ? & ? & Himp)".
         iExists s, succ, L1, L2, γ. iFrame.
-        iIntros "?". iApply "Himp". iFrame.
+        iIntros "(? & ?)". iApply "Himp". iFrame.
+    Qed.
+
+    Lemma list_equiv_insert (s n: loc) (head pred new succ: node_rep) 
+      (L: list node_rep) (γ': gname) (P: node_rep → iProp Σ) :
+      node_key new < node_key tail →
+      node_key pred < node_key new < node_key succ →
+      Sorted node_lt ([head] ++ L ++ [tail]) →
+      pred = head ∨ In pred L →
+      list_equiv ([head] ++ L) P ⊢ 
+        s ↦{#lfrac} rep_to_node succ
+        ∗ 
+        (node_next pred +ₗ lvl) ↦{#1/2} #s
+        ∗ 
+        (node_next new +ₗ lvl) ↦{#1/2} #s
+        ∗
+        inv (nodeN n) (node_inv n new)
+        ∗ 
+        n ↦{#lfrac} rep_to_node new
+        ∗ 
+        is_lock γ' (node_lock new) (in_lock (node_next new))
+        ∗
+        P new
+        -∗ 
+          ∃ (L' L1 L2: list node_rep), 
+            (node_next pred +ₗ lvl) ↦ #s
+            ∗
+            ⌜ [head] ++ L ++ [tail] = L1 ++ [pred; succ] ++ L2 ⌝
+            ∗
+            ⌜ Sorted node_lt ([head] ++ L' ++ [tail]) ⌝
+            ∗
+            ⌜ Permutation ([head] ++ L') ([head; new] ++ L) ⌝ 
+            ∗
+            ((node_next pred +ₗ lvl) ↦{#1/2} #n -∗ list_equiv ([head] ++ L') P).
+    Proof.
+      iIntros (Hnew Hrange Hsort Hin) .
+      iIntros "Hlist (Hs & Hpt & Hpt' & Hinvn & Hn & Hlock' & HP')".
+      remember ([head] ++ L) as L' eqn:HeqL'.
+      rewrite -in_inv in Hin.
+
+      iRevert (head L HeqL' Hsort Hin) "Hlist Hs Hpt Hpt' Hinvn Hn Hlock' HP'".
+      iInduction L' as [|pred'] "IHL'".
+      { iIntros (head L Hfalse); inversion Hfalse. }
+
+      iIntros (head L HeqL' Hsort).
+      inversion HeqL'; subst.
+      iIntros (Hin); inversion Hin as [Heq|HinL].
+      + subst.
+        iIntros "Hlist Hs Hpt Hpt' #Hinvn Hn #Hlock' HP'".
+        destruct L as [|succ' L].
+        - iDestruct "Hlist" as (γ t) "(Hpt'' & #Hinvt & Ht & #Hlock)".
+          iDestruct (mapsto_agree with "Hpt Hpt''") as %Heq.
+          assert (s = t) as -> by congruence.
+          iDestruct (mapsto_agree with "Hs Ht") as %->%rep_to_node_inj.
+          
+          iExists (new :: nil), nil, nil.
+          iFrame. iSplit; first done. iSplit.
+          { 
+            iPureIntro; apply Sorted_cons; econstructor.
+            auto. econstructor.
+            all: unfold node_lt; lia.
+          }
+          iSplit; first auto.
+          iIntros "Hpt". 
+          iExists γ, n. iFrame "# ∗".
+          iExists γ', t. iFrame "# ∗".
+        - iDestruct "Hlist" as (γ s') "(Hpt'' & #Hinvs' & Hs' & #Hlock & Hmatch)".
+          iDestruct (mapsto_agree with "Hpt Hpt''") as %Heq.
+          assert (s = s') as <- by congruence.
+          iDestruct (mapsto_agree with "Hs Hs'") as %<-%rep_to_node_inj.
+
+          iExists (new :: succ :: L), nil, (L ++ [tail]).
+          iFrame. iSplit; first done. iSplit.
+          { 
+            iPureIntro.
+            repeat apply Sorted_inv in Hsort as (Hsort&?).
+            repeat econstructor; auto. 
+            all: unfold node_lt; lia.
+          }
+          iSplit; first auto.
+          iIntros "Hpt". 
+          iExists γ, n. iFrame "# ∗".
+          iExists γ', s. iFrame "# ∗".
+      + destruct L as [|head' L]; first by inversion HinL.
+        iIntros "Hlist Hs Hpt Hpt' #Hinvn Hn #Hlock' HP'".
+
+        simpl in Hsort; apply Sorted_inv in Hsort as (Hsort&Hhd).
+        iDestruct "Hlist" as (γ h') "(Hpt'' & #Hinvh' & Hh' & Hlock & HP & Hmatch)".
+        iPoseProof ("IHL'" $! head' L with "[%] [%] [%] [$] [$] [$] [$] [$] [$] [$] [$]") 
+          as "Hclose"; auto.
+        
+        iDestruct "Hclose" as (L' L1 L2) "(Hpt' & %Hsplit & %Hsort' & %Hperm' & Himp')".
+        iExists (head' :: L'), (head :: L1), L2. iFrame.
+        iSplit.
+        {
+          rewrite /= in Hsplit.
+          rewrite /= Hsplit //.
+        }
+        iSplit.
+        {
+          iPureIntro. inversion Hhd.
+          apply Sorted_inv in Hsort' as (Hsort'&?).
+          repeat econstructor; auto.
+        }
+        iSplit.
+        {
+          iPureIntro. 
+          simpl in Hperm'; rewrite Hperm'. 
+          econstructor; econstructor.
+        }
+
+        iIntros "Hpt". iExists γ, h'.
+        iPoseProof ("Himp'" with "Hpt") as "Hlist".
+        iFrame "# ∗".
     Qed.
 
   End Proofs.
